order verification to be done

a1/selection_sort.dfy
@@ -1,48 +1,81 @@
 // (In place) Selection sort (in non-descending order) on integer arrays by traversing the unsorted
 // portion of the array from left to right and moving the maximum element to the right-most
 // unsorted place.
+predicate permutation (A:seq<int>, B:seq<int>) 
+{
+    multiset(A) == multiset(B)
+}
 
+predicate partOrdered(A:array<int>, lo:int, hi:int) 
+    // requires A != null
+    requires 0 <= lo <= hi <= A.Length
+    reads A
+{
+    forall i, j :: lo <= i < j < hi ==> A[i] <= A[j]
+}
+
+predicate ordered(A:array<int>)
+    // requires A != null
+    reads A
+{
+    partOrdered(A, 0, A.Length)
+}
 method selectionSort(a:array<int>)
 modifies a
+// ensures ordered(a)
+ensures permutation(a[..] , old(a[..]))
 {
     if a.Length > 1
     {
         var max, i : int;
         i := a.Length -1;
-        max := 0;
+        
+        // var sorted_idx := a.Length - 1;
+        max := i;
         while i > 0
-        invariant 0 <= i <= a.Length - 1
-        invariant 0 <= max
-        invariant max <= a.Length - 1
-        {
-            max := select(a, i);
+        invariant 0 <= i < a.Length
+        invariant permutation (a[..], old(a[..])) 
+        invariant 0 <= max < a.Length
+        // invariant partOrdered(a, i, a.Length)
+        decreases i
+        {   
+            print i, " ";
+            select(a, i); 
             // swap
-            a[i], a[max] := a[max], a[i];
+            // a[i], a[max] := a[max], a[i];
             i := i - 1;
+            print a[i..], "\n";
+            print i, " ";
         }
     }
+    print "\n";
 }
 
-method select(a:array<int>, idx:int) returns (m : int)
+// select max element from 0 to idx
+method select(a:array<int>, idx:int )// returns (max : int)
+modifies a
 requires 0 <= idx < a.Length
-requires a.Length > 0
-ensures 0 <= m < a.Length
+// ensures 0 <= max <= idx
+ensures forall x :: 0 <= x <= idx ==> a[x] <= a[idx]
+ensures permutation (a[..], old(a[..]))
+// ensures partOrdered(a, idx, a.Length)
 {
     var j := idx;
-    var max := 0;
+    var max := idx;
 
     while j > 0
     invariant 0 <= j <= idx
     invariant 0 <= max <= idx
+    invariant forall x :: j <= x <= idx ==> a[x] <= a[max]
+    invariant permutation (a[..], old(a[..])) 
     decreases j
     {
+        j := j-1;
         if a[j] > a[max] {
             max := j;
         }
-        j := j-1;
-
     }
-    m := max;
+    a[idx], a[max] := a[max], a[idx];
 
 }
 
